Update liveness logic: separate 'Lifetime RA' from the logic

src/example/Spinlock.v
@@ -76,27 +76,27 @@ Liveness chain of a spinlock :
    *)
 
   (** Invariants. *)
-  TODO (* Update live / dead *)
-  Definition spinlockInv (n : nat) (r : nat) (x : SCMem.val) (P : Formula n) (k l : nat)
+  Definition spinlockInv (n : nat) (γ : nat) (x : SCMem.val) (P : Formula n) (γk k l : nat)
     : Formula n :=
-    ((∃ (q : τ{Qp}) (u : τ{nat}),
-         ➢(@auexa_b r (Qp * nat)%type (q, u))
+    ((∃ (q : τ{Qp}) (γu u : τ{nat}),
+         ➢(@auexa_b γ (Qp * nat * nat)%type (q, γu, u))
           ∗
-          (((x ↦ 0) ∗ ◇[k](1 + l, 1) ∗ ➢(@auexa_w r (Qp * nat)%type (q, u)) ∗ P)
-           ∨ ((x ↦ 1) ∗ live[k] q ∗ live[u] (1/2) ∗ (-[u](0)-◇ emp) ∗ (u -(0)-◇ k))))
-     ∨ dead[k]
+          (((x ↦ 0) ∗ ◇[k](1 + l, 1) ∗ ➢(@auexa_w γ (Qp * nat * nat)%type (q, γu, u)) ∗ P)
+           ∨ ((x ↦ 1) ∗ ➢(@live γk nat k q) ∗ ➢(@live γu nat u (1/2)) ∗ (-[u](0)-◇ ➢(@dead γu nat u)) ∗ (u -(0)-◇ k))))
+     ∨ ➢(@dead γk nat k)
     )%F.
 
   (* Namespace for Spinlock invariants. *)
   Definition N_Spinlock : namespace := (nroot .@ "Spinlock").
 
-  Definition isSpinlock n (r : nat) (x : SCMem.val) (P : Formula n) (k L l : nat)
+  Definition isSpinlock n (γ : nat) (x : SCMem.val) (P : Formula n) (γk k L l : nat)
     : Formula n :=
     (∃ (N : τ{namespace, n}),
         (⌜(↑N ⊆ (↑N_Spinlock : coPset))⌝)
-          ∗ ◆[k, L] ∗ (⌜0 < l⌝) ∗ syn_inv n N (spinlockInv n r x P k l))%F.
+          ∗ ◆[k, L] ∗ (⌜0 < l⌝) ∗ syn_inv n N (spinlockInv n γ x P γk k l))%F.
 
-  Global Instance isSpinlock_persistent n r x P k L l : Persistent (⟦isSpinlock n r x P k L l, n⟧).
+  Global Instance isSpinlock_persistent n γ x P γk k L l :
+    Persistent (⟦isSpinlock n γ x P γk k L l, n⟧).
   Proof.
     unfold Persistent. iIntros "H". unfold isSpinlock. red_tl.
     iDestruct "H" as "[%N H]". iExists N. red_tl. rewrite red_syn_inv.
@@ -110,21 +110,21 @@ Liveness chain of a spinlock :
   Proof. apply ndot_ne_disjoint. ss. Qed.
 
   Lemma make_isSpinlock
-        n r x P k L l (LT : 0 < l)
-        (q : Qp) (u : nat) Es
+        n γ x P γk k L l (LT : 0 < l)
+        (q : Qp) (γu u : nat) Es
     :
     ⊢
-      ⟦((x ↦ 0) ∗ ➢(auexa_b r (q, u)) ∗ ➢(auexa_w r (q, u)) ∗ (⤉P) ∗ ◆[k, L] ∗ ◇[k](1+l, 1))%F, 1+n⟧
+      ⟦((x ↦ 0) ∗ ➢(auexa_b γ (q, γu, u)) ∗ ➢(auexa_w γ (q, γu, u)) ∗ (⤉P) ∗ ◆[k, L] ∗ ◇[k](1+l, 1))%F, 1+n⟧
         -∗
-        ⟦( =|1+n|={Es}=> (⤉(isSpinlock n r x P k L l)))%F, 1+n⟧.
+        ⟦( =|1+n|={Es}=> (⤉(isSpinlock n γ x P γk k L l)))%F, 1+n⟧.
   Proof.
     red_tl. simpl. iIntros "(PT & BQ & WQ & P & #LO & PC)".
     rewrite red_syn_fupd. red_tl.
-    iMod ((FUpd_alloc _ _ _ n (↑(N_Spinlock.@"a")) (spinlockInv n r x P k l))
+    iMod ((FUpd_alloc _ _ _ n (↑(N_Spinlock.@"a")) (spinlockInv n γ x P γk k l))
            with "[PT BQ WQ P PC]") as "#SINV".
     auto.
-    { simpl. unfold spinlockInv. red_tl. iLeft. iExists q. red_tl. iExists u. red_tl.
-      iSplitL "BQ". iFrame. iLeft. iFrame.
+    { simpl. unfold spinlockInv. red_tl. iLeft. iExists q. red_tl. iExists γu. red_tl. iExists u.
+      red_tl. iSplitL "BQ". iFrame. iLeft. iFrame.
     }
     iModIntro. unfold isSpinlock. red_tl.
     iExists (↑(N_Spinlock.@"a")). red_tl. iSplit.
@@ -133,34 +133,33 @@ Liveness chain of a spinlock :
   Qed.
 
   Lemma init_isSpinlock
-        n x P k L l (LT : 0 < l)
+        n x P γk k L l (LT : 0 < l)
         Es
     :
     ⊢
       ⟦(➢(auexa) ∗ (x ↦ 0) ∗ (⤉P) ∗ ◆[k, L] ∗ ◇[k](1+l, 1))%F, 1+n⟧
         -∗
-        ⟦( =|1+n|={Es}=> (➢(auexa) ∗ ∃ (r : τ{nat}), ⤉(isSpinlock n r x P k L l)))%F, 1+n⟧.
+        ⟦( =|1+n|={Es}=> (➢(auexa) ∗ ∃ (γ : τ{nat}), ⤉(isSpinlock n γ x P γk k L l)))%F, 1+n⟧.
   Proof.
     red_tl. simpl. iIntros "(AEA & PT & P & #LO & PC)".
     rewrite red_syn_fupd. red_tl.
-    iMod (auexa_alloc_gt _ ((1%Qp, 0)) with "AEA") as "[AEA (%r & BQ & BW)]".
-    iPoseProof (make_isSpinlock n r x P k L l with "[PT BQ BW P PC]") as "ISL".
+    iMod (auexa_alloc_gt _ ((1%Qp, 0, 0)) with "AEA") as "[AEA (%γ & BQ & BW)]".
+    iPoseProof (make_isSpinlock n γ x P γk k L l with "[PT BQ BW P PC]") as "ISL".
     auto.
     { red_tl. iFrame. iApply "LO". }
     iEval (rewrite red_syn_fupd) in "ISL". iMod "ISL".
-    iModIntro. iSplitL "AEA". iFrame.
-    iExists r. iFrame.
+    iModIntro. iSplitL "AEA". iFrame. iExists γ. iFrame.
   Qed.
 
   Lemma update_isSpinlock
-        n r x P k L l
+        n γ x P γk k L l
         Es
         (MASK_SL : mask_has_Spinlock Es n)
-        k' L' l' (LT' : 0 < l')
+        γk' k' L' l' (LT' : 0 < l')
     :
-    ⊢⟦((⤉(isSpinlock n r x P k L l)) ∗ live[k] 1 ∗ ◆[k', L'] ∗ ◇[k'](1+ l', 1))%F, 1+n⟧
+    ⊢ ⟦((⤉(isSpinlock n γ x P γk k L l)) ∗ ➢(live γk k 1) ∗ ◆[k', L'] ∗ ◇[k'](1+ l', 1))%F, 1+n⟧
        -∗
-       ⟦( =|1+n|={Es}=>((⤉ isSpinlock n r x P k' L' l') ∗ dead[k]))%F, 1+n⟧.
+       ⟦( =|1+n|={Es}=>((⤉ isSpinlock n γ x P γk' k' L' l') ∗ ➢(dead γk k)))%F, 1+n⟧.
   Proof.
     red_tl. simpl. iIntros "(ISL & LIVE & LO' & PC')". rewrite red_syn_fupd. red_tl.
     iEval (unfold isSpinlock) in "ISL". red_tl.
@@ -170,18 +169,18 @@ Liveness chain of a spinlock :
     { unfold mask_has_Spinlock in MASK_SL. des_ifs. set_solver. }
     simpl. iEval (unfold spinlockInv; red_tl) in "SI".
     iDestruct "SI" as "[[%q SI] | DEAD]".
-    2:{ iExFalso. simpl. iPoseProof (not_dead with "[LIVE DEAD]") as "F". iFrame. auto. }
-    red_tl. iDestruct "SI" as "[%u SI]".
+    2:{ iExFalso. simpl. iPoseProof (Lifetime.pending_not_shot with "LIVE DEAD") as "F". auto. }
+    red_tl. iDestruct "SI" as "[%γu SI]". red_tl. iDestruct "SI" as "[%u SI]".
     red_tl. iDestruct "SI" as "[BQ [(PT & _ & WQ & P) | (_ & LIVE2 & _)]]".
-    2:{ iPoseProof (live_merge with "[LIVE2 LIVE]") as "LIVE". iFrame.
-        iPoseProof (live_wf with "LIVE") as "%F". exfalso. eapply Qp_add_lt_one. eauto.
+    2:{ iPoseProof (Lifetime.pending_merge with "LIVE LIVE2") as "LIVE".
+        iPoseProof (Lifetime.pending_wf with "LIVE") as "%F". exfalso.
+        eapply Qp_add_lt_one. eauto.
     }
-    iMod (kill with "LIVE") as "#DEAD". iMod ("K" with "[DEAD]") as "_".
+    iMod (Lifetime.pending_shot with "LIVE") as "#DEAD". iMod ("K" with "[DEAD]") as "_".
     { unfold spinlockInv. red_tl. iRight. eauto. }
-    iPoseProof (make_isSpinlock n r x P k' L' l' LT' with "[PT BQ WQ P LO' PC']") as "ISL".
+    iPoseProof (make_isSpinlock n γ x P γk' k' L' l' LT' with "[PT BQ WQ P LO' PC']") as "ISL".
     { red_tl. iFrame. }
-    rewrite red_syn_fupd. iMod "ISL".
-    iModIntro. iFrame. auto.
+    rewrite red_syn_fupd. iMod "ISL". iModIntro. iFrame. auto.
   Qed.
 
   Lemma Spinlock_lock_spec
@@ -190,19 +189,19 @@ Liveness chain of a spinlock :
         (MASK_TOP : OwnEs_top Es)
         (MASK_STTGT : mask_has_st_tgt Es n)
     :
-    ⊢ ∀ r x (P : Formula n) k L l q (ds : list (nat * nat * Formula n)),
+    ⊢ ∀ γ x (P : Formula n) γk k L l q (ds : list (nat * nat * Formula n)),
         [@ tid, n, Es @]
           ⧼⟦(((syn_tgt_interp_as n sndl (fun m => (➢ (scm_memory_black m))))
-                ∗ (⤉ isSpinlock n r x P k L l)
-                ∗ live[k] q ∗ (⤉ Duty(tid) ds)
+                ∗ (⤉ isSpinlock n γ x P γk k L l)
+                ∗ ➢(live γk k q) ∗ (⤉ Duty(tid) ds)
                 ∗ ◇{List.map fst ds}(2 + L, 1))%F), 1+n⟧⧽
             (OMod.close_itree Client (SCMem.mod gvs) (Spinlock.lock x))
-            ⧼rv, ⟦(∃ (u : τ{nat, 1+n}),
-                      (⤉ P) ∗ ➢(auexa_w r (((q/2)%Qp, u) : Qp * nat)) ∗ live[k] (q/2)
-                       ∗ (⤉ Duty(tid) ((u, 0, emp) :: ds)) ∗ live[u] (1/2) ∗ ◇[u](l, 1))%F, 1+n⟧⧽
+            ⧼rv, ⟦(∃ (γu u : τ{nat, 1+n}),
+                      (⤉ P) ∗ ➢(auexa_w γ (((q/2)%Qp, γu, u) : Qp * nat * nat)) ∗ ➢(live γk k (q/2))
+                       ∗ (⤉ Duty(tid) ((u, 0, ➢(@dead γu nat u)) :: ds)) ∗ ➢(@live γu nat u (1/2)) ∗ ◇[u](l, 1))%F, 1+n⟧⧽
   .
   Proof.
-    iIntros (? ? ? ? ? ? ? ?).
+    iIntros (? ? ? ? ? ? ? ? ?).
     iStartTriple. iIntros "PRE POST". unfold Spinlock.lock.
     (* Preprocess for induction. *)
     iApply wpsim_free_all. auto.
@@ -227,7 +226,8 @@ Liveness chain of a spinlock :
     (* Case analysis on lock variable. *)
     iInv "INV" as "SLI" "SLI_CLOSE". iEval (unfold spinlockInv; simpl; red_tl; simpl) in "SLI".
     iDestruct "SLI" as "[[%q0 SLI] | DEAD]".
-    2:{ iExFalso. iPoseProof (not_dead with "[LIVE DEAD]") as "%F". iFrame. auto. }
+    2:{ iExFalso. iPoseProof (Lifetime.pending_not_shot with "LIVE DEAD") as "%F". iFrame. auto. }
+    iEval (red_tl; simpl) in "SLI". iDestruct "SLI" as "[%γu0 SLI]".
     iEval (red_tl; simpl) in "SLI". iDestruct "SLI" as "[%u0 SLI]".
     iEval (red_tl; simpl) in "SLI". iDestruct "SLI" as "[qISB [ACQ|WAIT]]".
 
@@ -245,33 +245,35 @@ Liveness chain of a spinlock :
       clear e. des. subst. rred2r. iApply wpsim_tauR. rred2r.
       (* Close the invariant spinlockInv: *)
       (* 1. Allocate new obligation: I will release the lock. *)
-      iMod (alloc_obligation l 2) as "(%k1 & #LO1 & PC1 & LIVE1)".
+      iMod (alloc_obligation l 2) as "(%k1 & #LO1 & PC1)".
+      iMod (Lifetime.alloc k1) as "[%γk1 LIVE1]".
       (* 2. Preprocess. *)
-      iPoseProof (live_split _ (1/2)%Qp (1/2)%Qp with "[LIVE1]") as "[LIVE1 LIVE1']".
+      iPoseProof (Lifetime.pending_split _ (1/2)%Qp (1/2)%Qp with "[LIVE1]") as "[LIVE1 LIVE1']".
       { iEval (rewrite Qp.half_half). iFrame. }
       iEval (replace 2 with (1+1) by lia) in "PC1".
       iPoseProof (pc_split with "PC1") as "[PC1 PC_POST]".
       iMod (pc_mon _ 1 _ 1 _ _ with "PC1") as "PC1". Unshelve.
       2:{ apply layer_drop_eq; auto. }
-      iMod (duty_add _ _ _ _ 0 (emp%F : Formula n) with "[DUTY PC1] []") as "DUTY".
+      iMod (duty_add _ _ _ _ 0 ((➢ dead γk1 k1)%F : Formula n) with "[DUTY PC1] []") as "DUTY".
       { iFrame. }
       { iModIntro. iEval (ss; red_tl). auto. }
       iPoseProof (duty_tpromise with "DUTY") as "#PROM1".
       { simpl. left. auto. }
       iMod (link_new k1 k l 0 0 with "[PCk]") as "[#LINK1 _]".
       { iFrame. eauto. }
-      iPoseProof ((live_split k (q/2)%Qp (q/2)%Qp) with "[LIVE]") as "[MYLIVE LIVE]".
+      iPoseProof ((Lifetime.pending_split _ (q/2)%Qp (q/2)%Qp) with "[LIVE]") as "[MYLIVE LIVE]".
       { rewrite Qp.div_2. iFrame. }
       iMod (auexa_b_w_update with "qISB qISW") as "[qISB qISW]".
       (* Now close with SLI_CLOSE. *)
       iMod ("SLI_CLOSE" with "[LIVE PT LIVE1' qISB]") as "_".
       { iEval (unfold spinlockInv; simpl; red_tl; simpl).
-        iLeft. iExists (q/2)%Qp. iEval (red_tl; simpl). iExists k1. iEval (red_tl; simpl).
-        iSplitL "qISB"; [iFrame|].
-        iRight. iFrame. auto.
+        iLeft. iExists (q/2)%Qp.
+        iEval (red_tl; simpl). iExists γk1. iEval (red_tl; simpl). iExists k1. iEval (red_tl; simpl).
+        iSplitL "qISB"; [iFrame|]. iRight. iFrame. auto.
       }
       (* Finish with POST. *)
-      iApply "POST". iEval (red_tl; simpl). iExists k1. iEval (red_tl; simpl). iFrame.
+      iApply "POST". iEval (red_tl; simpl). iExists γk1. iEval (red_tl; simpl). iExists k1.
+      iEval (red_tl; simpl). iFrame.
     }
 
     (** Case 2. Miss the lock and loops. *)
@@ -287,18 +289,18 @@ Liveness chain of a spinlock :
       { exfalso. ss. }
       clear n0. des. subst. rred2r. iApply wpsim_tauR. rred2r. iApply wpsim_tauR.
       (* Get credits from IH and the invariant. *)
-      iMod (tpromise_progress with "[FC]") as "[PC | [DEAD _]]".
+      iMod (tpromise_progress with "[FC]") as "[PC | DEAD]".
       { iFrame. iApply "OATH". }
-      2:{ iExFalso. iPoseProof (not_dead with "[LIVE_O DEAD]") as "%FALSE". iFrame. auto. }
+      2:{ iExFalso. iPoseProof (Lifetime.pending_not_shot with "LIVE_O DEAD") as "%FALSE". auto. }
       iMod (link_amplify with "[PC]") as "PC".
       { iFrame. iApply "LINK". }
       iMod ("IH" with "PC") as "IH".
       (* Close the invariant spinlockInv. *)
       iMod ("SLI_CLOSE" with "[qISB LIVE_SL LIVE_O PT]") as "_".
       { iEval (unfold spinlockInv; simpl; red_tl; simpl).
-        iLeft. iExists q0. iEval (red_tl; simpl). iExists u0. iEval (red_tl; simpl).
-        iSplitL "qISB"; [iFrame|].
-        iRight. iFrame. auto.
+        iLeft. iExists q0. iEval (red_tl; simpl).
+        iExists γu0. iEval (red_tl; simpl). iExists u0. iEval (red_tl; simpl).
+        iSplitL "qISB"; [iFrame|]. iRight. iFrame. auto.
       }
       (* Finish with IH. *)
       iApply wpsim_stutter_mon. i; eauto. instantiate (1:=pt). i; auto.
@@ -310,39 +312,40 @@ Liveness chain of a spinlock :
         tid n
         (Es : coPsets)
     :
-    ⟦(∀ (r : τ{nat})
+    ⟦(∀ (γ : τ{nat})
         (x : τ{SCMem.val})
         (P : τ{Φ, 1+n})
-        (k L l : τ{nat})
+        (γk k L l : τ{nat})
         (q : τ{Qp})
         (ds : τ{ listT (nat * nat * Φ)%ftype, 1+n})
        ,
          [@ tid, n, Es @]
            ⧼((syn_tgt_interp_as n sndl (fun m => (➢ (scm_memory_black m))))
-                ∗ (⤉ isSpinlock n r x P k L l)
-                ∗ live[k] q ∗ (⤉ Duty(tid) ds)
+                ∗ (⤉ isSpinlock n γ x P γk k L l)
+                ∗ ➢(@live γk nat k q) ∗ (⤉ Duty(tid) ds)
                 ∗ ◇{List.map fst ds}(2 + L, 1))⧽
              (OMod.close_itree Client (SCMem.mod gvs) (Spinlock.lock x))
-             ⧼rv, (∃ (u : τ{nat, 1+n}),
-                      (⤉ P) ∗ ➢(auexa_w r (((q/2)%Qp, u) : Qp * nat)) ∗ live[k] (q/2)
-                            ∗ (⤉ Duty(tid) ((u, 0, emp) :: ds)) ∗ live[u] (1/2) ∗ ◇[u](l, 1))⧽)%F, 1+n⟧
+             ⧼rv, (∃ (γu u : τ{nat, 1+n}),
+                      (⤉ P) ∗ ➢(auexa_w γ (((q/2)%Qp, γu, u) : Qp * nat * nat)) ∗ ➢(@live γk nat k (q/2))
+                            ∗ (⤉ Duty(tid) ((u, 0, ➢(@dead γu nat u)) :: ds)) ∗ ➢(@live γu nat u (1/2)) ∗ ◇[u](l, 1))⧽)%F, 1+n⟧
     =
-      (∀ r x (P : Formula n) k L l q (ds : list (nat * nat * Formula n)),
+      (∀ γ x (P : Formula n) γk k L l q (ds : list (nat * nat * Formula n)),
           [@ tid, n, Es @]
             ⧼⟦((syn_tgt_interp_as n sndl (fun m => (➢ (scm_memory_black m))))
-                  ∗ (⤉ isSpinlock n r x P k L l)
-                  ∗ live[k] q ∗ (⤉ Duty(tid) ds)
+                  ∗ (⤉ isSpinlock n γ x P γk k L l)
+                  ∗ ➢(live γk k q) ∗ (⤉ Duty(tid) ds)
                   ∗ ◇{List.map fst ds}(2 + L, 1))%F, 1+n⟧⧽
               (OMod.close_itree Client (SCMem.mod gvs) (Spinlock.lock x))
-              ⧼rv, ⟦(∃ (u : τ{nat, 1+n}),
-                        (⤉ P) ∗ ➢(auexa_w r (((q/2)%Qp, u) : Qp * nat)) ∗ live[k] (q/2)
-                              ∗ (⤉ Duty(tid) ((u, 0, emp) :: ds)) ∗ live[u] (1/2) ∗ ◇[u](l, 1))%F, 1+n⟧⧽)%I
+              ⧼rv, ⟦(∃ (γu u : τ{nat, 1+n}),
+                        (⤉ P) ∗ ➢(auexa_w γ (((q/2)%Qp, γu, u) : Qp * nat * nat)) ∗ ➢(live γk k (q/2))
+                              ∗ (⤉ Duty(tid) ((u, 0, ➢(@dead γu nat u)) :: ds)) ∗ ➢(@live γu nat u (1/2)) ∗ ◇[u](l, 1))%F, 1+n⟧⧽)%I
   .
   Proof.
     simpl.
-    red_tl. apply f_equal. extensionalities r.
+    red_tl. apply f_equal. extensionalities γ.
     red_tl. apply f_equal. extensionalities x.
     red_tl. apply f_equal. extensionalities P.
+    red_tl. apply f_equal. extensionalities γk.
     red_tl. apply f_equal. extensionalities k.
     red_tl. apply f_equal. extensionalities L.
     red_tl. apply f_equal. extensionalities l.
@@ -357,22 +360,22 @@ Liveness chain of a spinlock :
         (MASK_TOP : OwnEs_top Es)
         (MASK_STTGT : mask_has_st_tgt Es n)
     :
-    ⊢ ⟦(∀ (r : τ{nat})
+    ⊢ ⟦(∀ (γ : τ{nat})
           (x : τ{SCMem.val})
           (P : τ{Φ, 1+n})
-          (k L l : τ{nat})
+          (γk k L l : τ{nat})
           (q : τ{Qp})
           (ds : τ{ listT (nat * nat * Φ)%ftype, 1+n})
          ,
            [@ tid, n, Es @]
              ⧼((syn_tgt_interp_as n sndl (fun m => (➢ (scm_memory_black m))))
-                  ∗ (⤉ isSpinlock n r x P k L l)
-                  ∗ live[k] q ∗ (⤉ Duty(tid) ds)
+                  ∗ (⤉ isSpinlock n γ x P γk k L l)
+                  ∗ ➢(@live γk nat k q) ∗ (⤉ Duty(tid) ds)
                   ∗ ◇{List.map fst ds}(2 + L, 1))⧽
                (OMod.close_itree Client (SCMem.mod gvs) (Spinlock.lock x))
-               ⧼rv, (∃ (u : τ{nat, 1+n}),
-                        (⤉ P) ∗ ➢(auexa_w r (((q/2)%Qp, u) : Qp * nat)) ∗ live[k] (q/2)
-                              ∗ (⤉ Duty(tid) ((u, 0, emp) :: ds)) ∗ live[u] (1/2) ∗ ◇[u](l, 1))⧽)%F, 1+n⟧
+               ⧼rv, (∃ (γu u : τ{nat, 1+n}),
+                        (⤉ P) ∗ ➢(auexa_w γ (((q/2)%Qp, γu, u) : Qp * nat * nat)) ∗ ➢(@live γk nat k (q/2))
+                              ∗ (⤉ Duty(tid) ((u, 0, ➢(@dead γu nat u)) :: ds)) ∗ ➢(@live γu nat u (1/2)) ∗ ◇[u](l, 1))⧽)%F, 1+n⟧
   .
   Proof.
     rewrite red_syn_Spinlock_lock_spec. iApply Spinlock_lock_spec. all: auto.
@@ -384,19 +387,19 @@ Liveness chain of a spinlock :
         (MASK_TOP : OwnEs_top Es)
         (MASK_STTGT : mask_has_st_tgt Es n)
     :
-    ⊢ ∀ r x (P : Formula n) k L l q (ds : list (nat * nat * Formula n)) u,
+    ⊢ ∀ γ x (P : Formula n) γk k L l q (ds : list (nat * nat * Formula n)) γu u,
         [@ tid, n, Es @]
           ⧼⟦(((syn_tgt_interp_as n sndl (fun m => (➢ (scm_memory_black m))))
-                ∗ (⤉ isSpinlock n r x P k L l) ∗ (⤉ P)
-                ∗ ➢(auexa_w r (((q/2)%Qp, u) : Qp * nat)) ∗ live[k] (q/2)
-                ∗ (⤉ Duty(tid) ((u, 0, emp) :: ds)) ∗ live[u] (1/2)
-                ∗ ◇{List.map fst ((u, 0, emp) :: ds)}(1, 1)
+                ∗ (⤉ isSpinlock n γ x P γk k L l) ∗ (⤉ P)
+                ∗ ➢(auexa_w γ (((q/2)%Qp, γu, u) : Qp * nat * nat)) ∗ ➢(live γk k (q/2))
+                ∗ (⤉ Duty(tid) ((u, 0, ➢(dead γu u)) :: ds)) ∗ ➢(live γu u (1/2))
+                ∗ ◇{List.map fst ((u, 0, ➢(dead γu u)) :: ds)}(1, 1)
                 ∗ ◇[k](1 + l, 1)))%F, 1+n⟧⧽
             (OMod.close_itree Client (SCMem.mod gvs) (Spinlock.unlock x))
-            ⧼rv, ⟦((⤉ Duty(tid) ds) ∗ live[k] q)%F, 1+n⟧⧽
+            ⧼rv, ⟦((⤉ Duty(tid) ds) ∗ ➢(live γk k q))%F, 1+n⟧⧽
   .
   Proof.
-    iIntros (? ? ? ? ? ? ? ? ?).
+    iIntros (? ? ? ? ? ? ? ? ? ? ?).
     iStartTriple. iIntros "PRE POST". unfold Spinlock.unlock.
     (* Preprocess. *)
     iApply wpsim_free_all. auto.
@@ -412,7 +415,8 @@ Liveness chain of a spinlock :
     (* Open invariant. *)
     iInv "INV" as "SLI" "SLI_CLOSE". iEval (unfold spinlockInv; simpl; red_tl; simpl) in "SLI".
     iDestruct "SLI" as "[[%q0 SLI] | DEAD]".
-    2:{ iExFalso. iPoseProof (not_dead with "[LIVE DEAD]") as "%F". iFrame. auto. }
+    2:{ iExFalso. iPoseProof (Lifetime.pending_not_shot with "LIVE DEAD") as "%F". auto. }
+    iEval (red_tl; simpl) in "SLI". iDestruct "SLI" as "[%γu0 SLI]".
     iEval (red_tl; simpl) in "SLI". iDestruct "SLI" as "[%u0 SLI]".
     iEval (red_tl; simpl) in "SLI". iDestruct "SLI" as "[BQ [ACQ | WAIT]]".
     { iExFalso. iDestruct "ACQ" as "(_ & _ & WQ2 & _)".
@@ -428,60 +432,62 @@ Liveness chain of a spinlock :
     iPoseProof (auexa_b_w_eq with "BQ WQ") as "%EQ". clarify.
     iMod ("SLI_CLOSE" with "[P WQ PCk BQ PT]") as "_".
     { simpl. iEval (unfold spinlockInv). red_tl. iLeft.
-      iExists (q/2)%Qp. red_tl. iExists u. red_tl. iSplitL "BQ". iFrame. iLeft. iFrame.
+      iExists (q/2)%Qp. red_tl. iExists γu. red_tl. iExists u.
+      red_tl. iSplitL "BQ". iFrame. iLeft. iFrame.
     }
     (* Postconditions. *)
-    iMod (kill with "[LIVEU LIVEU2]") as "DEADU".
-    { iEval (rewrite <- Qp.half_half). iApply live_merge. iFrame. }
+    iMod (Lifetime.pending_shot with "[LIVEU LIVEU2]") as "#DEADU".
+    { iEval (rewrite <- Qp.half_half). iApply (Lifetime.pending_merge with "LIVEU LIVEU2"). }
     iMod (duty_fulfill with "[DUTY DEADU]") as "DUTY".
-    { iFrame. }
-    iPoseProof (live_merge with "[LIVE LIVE2]") as "LIVE". iFrame. iEval (rewrite Qp.div_2) in "LIVE".
-    iApply "POST". red_tl. iFrame.
+    { iFrame. auto. }
+    iPoseProof (Lifetime.pending_merge with "LIVE LIVE2") as "LIVE".
+    iEval (rewrite Qp.div_2) in "LIVE". iApply "POST". red_tl. iFrame.
   Qed.
 
   Lemma red_syn_Spinlock_unlock_spec
         tid n
         (Es : coPsets)
     :
-    ⟦(∀ (r : τ{nat})
+    ⟦(∀ (γ : τ{nat})
         (x : τ{SCMem.val})
         (P : τ{Φ, 1+n})
-        (k L l : τ{nat})
+        (γk k L l : τ{nat})
         (q : τ{Qp})
         (ds : τ{ listT (nat * nat * Φ)%ftype, 1+n})
-        (u : τ{nat, 1+n})
+        (γu u : τ{nat, 1+n})
        ,
          [@ tid, n, Es @]
            ⧼((syn_tgt_interp_as n sndl (fun m => (➢(scm_memory_black m))))
-               ∗ (⤉ isSpinlock n r x P k L l) ∗ (⤉ P)
-               ∗ ➢(auexa_w r (((q/2)%Qp, u) : Qp * nat)) ∗ live[k] (q/2)
-               ∗ (⤉ Duty(tid) ((u, 0, emp) :: ds)) ∗ live[u] (1/2)
-               ∗ ◇{List.map fst ((u, 0, emp) :: ds)}(1, 1)
+               ∗ (⤉ isSpinlock n γ x P γk k L l) ∗ (⤉ P)
+               ∗ ➢(auexa_w γ (((q/2)%Qp, γu, u) : Qp * nat * nat)) ∗ ➢(@live γk nat k (q/2))
+               ∗ (⤉ Duty(tid) ((u, 0, ➢(@dead γu nat u)) :: ds)) ∗ ➢(@live γu nat u (1/2))
+               ∗ ◇{List.map fst ((u, 0, ➢(@dead γu nat u)) :: ds)}(1, 1)
                ∗ ◇[k](1 + l, 1))⧽
              (OMod.close_itree Client (SCMem.mod gvs) (Spinlock.unlock x))
-             ⧼rv, ((⤉ Duty(tid) ds) ∗ live[k] q)⧽)%F, 1+n⟧
+             ⧼rv, ((⤉ Duty(tid) ds) ∗ ➢(@live γk nat k q))⧽)%F, 1+n⟧
     =
-      (∀ r x (P : Formula n) k L l q (ds : list (nat * nat * Formula n)) u,
+      (∀ γ x (P : Formula n) γk k L l q (ds : list (nat * nat * Formula n)) γu u,
           [@ tid, n, Es @]
             ⧼⟦(((syn_tgt_interp_as n sndl (fun m => (➢ (scm_memory_black m))))
-                  ∗ (⤉ isSpinlock n r x P k L l) ∗ (⤉ P)
-                  ∗ ➢(auexa_w r (((q/2)%Qp, u) : Qp * nat)) ∗ live[k] (q/2)
-                  ∗ (⤉ Duty(tid) ((u, 0, emp) :: ds)) ∗ live[u] (1/2)
-                  ∗ ◇{List.map fst ((u, 0, emp) :: ds)}(1, 1)
+                  ∗ (⤉ isSpinlock n γ x P γk k L l) ∗ (⤉ P)
+                  ∗ ➢(auexa_w γ (((q/2)%Qp, γu, u) : Qp * nat * nat)) ∗ ➢(live γk k (q/2))
+                  ∗ (⤉ Duty(tid) ((u, 0, ➢(dead γu u)) :: ds)) ∗ ➢(live γu u (1/2))
+                  ∗ ◇{List.map fst ((u, 0, ➢(dead γu u)) :: ds)}(1, 1)
                   ∗ ◇[k](1 + l, 1)))%F, 1+n⟧⧽
               (OMod.close_itree Client (SCMem.mod gvs) (Spinlock.unlock x))
-              ⧼rv, ⟦((⤉ Duty(tid) ds) ∗ live[k] q)%F, 1+n⟧⧽)%I
+              ⧼rv, ⟦((⤉ Duty(tid) ds) ∗ ➢(live γk k q))%F, 1+n⟧⧽)%I
   .
   Proof.
-    (* simpl. *)
-    red_tl. apply f_equal. extensionalities r.
+    red_tl. apply f_equal. extensionalities γ.
     red_tl. apply f_equal. extensionalities x.
     red_tl. apply f_equal. extensionalities P.
+    red_tl. apply f_equal. extensionalities γk.
     red_tl. apply f_equal. extensionalities k.
     red_tl. apply f_equal. extensionalities L.
     red_tl. apply f_equal. extensionalities l.
     red_tl. apply f_equal. extensionalities q.
     red_tl. apply f_equal. extensionalities ds.
+    rewrite @red_tl_univ. apply f_equal. extensionalities γu.
     rewrite @red_tl_univ. apply f_equal. extensionalities u.
     apply red_syn_non_atomic_triple.
   Qed.
@@ -492,23 +498,23 @@ Liveness chain of a spinlock :
         (MASK_TOP : OwnEs_top Es)
         (MASK_STTGT : mask_has_st_tgt Es n)
     :
-    ⊢ ⟦(∀ (r : τ{nat})
+    ⊢ ⟦(∀ (γ : τ{nat})
           (x : τ{SCMem.val})
           (P : τ{Φ, 1+n})
-          (k L l : τ{nat})
+          (γk k L l : τ{nat})
           (q : τ{Qp})
           (ds : τ{ listT (nat * nat * Φ)%ftype, 1+n})
-          (u : τ{nat, 1+n})
+          (γu u : τ{nat, 1+n})
          ,
            [@ tid, n, Es @]
              ⧼((syn_tgt_interp_as n sndl (fun m => (➢(scm_memory_black m))))
-                 ∗ (⤉ isSpinlock n r x P k L l) ∗ (⤉ P)
-                 ∗ ➢(auexa_w r (((q/2)%Qp, u) : Qp * nat)) ∗ live[k] (q/2)
-                 ∗ (⤉ Duty(tid) ((u, 0, emp) :: ds)) ∗ live[u] (1/2)
-                 ∗ ◇{List.map fst ((u, 0, emp) :: ds)}(1, 1)
+                 ∗ (⤉ isSpinlock n γ x P γk k L l) ∗ (⤉ P)
+                 ∗ ➢(auexa_w γ (((q/2)%Qp, γu, u) : Qp * nat * nat)) ∗ ➢(@live γk nat k (q/2))
+                 ∗ (⤉ Duty(tid) ((u, 0, ➢(@dead γu nat u)) :: ds)) ∗ ➢(@live γu nat u (1/2))
+                 ∗ ◇{List.map fst ((u, 0, ➢(@dead γu nat u )) :: ds)}(1, 1)
                  ∗ ◇[k](1 + l, 1))⧽
                (OMod.close_itree Client (SCMem.mod gvs) (Spinlock.unlock x))
-               ⧼rv, ((⤉ Duty(tid) ds) ∗ live[k] q)⧽)%F, 1+n⟧
+               ⧼rv, ((⤉ Duty(tid) ds) ∗ ➢(@live γk nat k q))⧽)%F, 1+n⟧
   .
   Proof.
     rewrite red_syn_Spinlock_unlock_spec. iApply Spinlock_unlock_spec. all: auto.
